added explanation of why CPS is useful

src/NewBaseSystem.v
@@ -10,6 +10,249 @@ Require Import Crypto.Util.CPSUtil Crypto.Util.Prod.
 Require Import Coq.Lists.List. Import ListNotations.
 Require Crypto.Util.Tuple. Local Notation tuple := Tuple.tuple.
 
+(*****
+
+This file provides a generalized version of arithmetic with "mixed
+radix" numerical systems. Later, parameters are entered into the
+general functions, and they are partially evaluated until only runtime
+basic arithmetic operations remain.
+
+CPS
+---
+
+Fuctions are written in continuation passing style (CPS). This means
+that each operation is passed a "continuation" function, which it is
+expected to call on its own output (like a callback). See the end of
+this comment for a motivating example explaining why we do CPS,
+despite a fair amount of resulting boilerplate code for each
+operation. The code block for an operation called A would look like
+this:
+
+```
+Definition A_cps x y {T} f : T := ...
+
+Definition A x y := A_cps x y id.
+Lemma A_cps_id x y : forall {T} f, @A_cps x y T f = f (A x y).
+Hint Opaque A : uncps.
+Hint Rewrite A_cps_id : uncps.
+
+Lemma eval_A x y : eval (A x y) = ...
+Hint Rewrite eval_A : push_basesystem_eval.
+```
+
+`A_cps` is the main, CPS-style definition of the operation (`f` is the
+continuation function). `A` is the non-CPS version of `A_cps`, simply
+defined by passing an identity function to `A_cps`. `A_cps_id` states
+that we can replace the CPS version with the non-cps version. `eval_A`
+is the actual correctness lemma for the operation, stating that it has
+the correct arithmetic properties. In general, the middle block
+containing `A` and `A_cps_id` is boring boilerplate and can be safely
+ignored.
+
+HintDbs
+-------
+
++ `uncps` : Converts CPS operations to their non-CPS versions.
++ `push_basesystem_eval` : Contains all the correctness lemmas for
+   operations in this file, which are in terms of the `eval` function.
+
+Positional/Associational
+------------------------
+
+We represent mixed-radix numbers in a few different ways:
+
++ "Positional" : a tuple of numbers and a weight function (nat->Z),
+which is evaluated by multiplying the `i`th element of the tuple by
+`weight i`, and then summing the products.
++ "Associational" : a list of pairs of numbers--the first is the
+weight, the second is the runtime value. Evaluated by multiplying each
+pair and summing the products.
+
+The associational representation is good for basic operations like
+addition and multiplication; for addition, one can simply just append
+two associational lists. But the end-result code should use the
+positional representation (with each digit representing a machine
+word). Since converting to and fro can be easily compiled away once
+the weight function is known, we use associational to write most of
+the operations and liberally convert back and forth to ensure correct
+output. In particular, it is important to convert before carrying.
+
+Runtime Operations
+------------------
+
+Since some instances of e.g. Z.add or Z.mul operate on (compile-time)
+weights, and some operate on runtime values, we need a way to
+differentiate these cases before partial evaluation. We define a
+runtime_scope to mark certain additions/multiplications as runtime
+values, so they will not be unfolded during partial evaluation. For
+instance, if we have:
+
+```
+Definition f (x y : Z * Z) := (fst x + fst y, (snd x + snd y)%RT).
+```
+
+then when we are partially evaluating `f`, we can easily exclude the
+runtime operations (`cbv - [runtime_add]`) and prevent Coq from trying
+to simplify the second addition.
+
+
+Why CPS?
+--------
+
+Let's suppose we want to add corresponding elements of two `list Z`s
+(so on inputs `[1,2,3]` and `[2,3,1]`, we get `[3,5,4]`). We might
+write our function like this :
+
+```
+Fixpoint add_lists (p q : list Z) :=
+  match p, q with
+  | p0 :: p', q0 :: q' =>
+    dlet sum := p0 + q0 in
+    sum :: add_lists p' q'
+  | _, _ => nil
+  end.
+```
+
+(Note : `dlet` is a notation for `Let_In`, which is just a dumb
+wrapper for `let`. This allows us to `cbv - [Let_In]` if we want to
+not simplify certain `let`s.)
+
+A CPS equivalent of `add_lists` would look like this:
+
+```
+Fixpoint add_lists_cps (p q : list Z) {T} (f:list Z->T) :=
+  match p, q with
+  | p0 :: p', q0 :: q' =>
+    dlet sum := p0 + q0 in
+    add_lists_cps p' q' (fun r => f (sum :: r))
+  | _, _ => f nil
+  end.
+```
+
+Now let's try some partial evaluation. The expression we'll evaluate is:
+
+```
+Definition x := 
+    (fun a0 a1 a2 b0 b1 b2 =>
+      let r := add_lists [a0;a1;a2] [b0;b1;b2] in
+      let rr := add_lists r r in
+      add_lists rr rr).
+```
+
+Or, using `add_lists_cps`:
+
+```
+Definition y := 
+    (fun a0 a1 a2 b0 b1 b2 =>
+      add_lists_cps [a0;a1;a2] [b0;b1;b2]
+                     (fun r => add_lists_cps r r
+                     (fun rr => add_lists_cps rr rr id))).
+```
+
+If we run `Eval cbv -[Z.add] in x` and `Eval cbv -[Z.add] in y`, we get
+identical output:
+
+```
+fun a0 a1 a2 b0 b1 b2 : Z =>
+       [a0 + b0 + (a0 + b0) + (a0 + b0 + (a0 + b0));
+       a1 + b1 + (a1 + b1) + (a1 + b1 + (a1 + b1));
+       a2 + b2 + (a2 + b2) + (a2 + b2 + (a2 + b2))]
+```
+
+However, there are a lot of common subexpressions here--this is what
+the `dlet` we put into the functions should help us avoid. Let's try
+`Eval cbv -[Let_In Z.add] in x`:
+
+```
+fun a0 a1 a2 b0 b1 b2 : Z =>
+       (fix add_lists (p q : list Z) {struct p} : 
+        list Z :=
+          match p with
+          | [] => []
+          | p0 :: p' =>
+              match q with
+              | [] => []
+              | q0 :: q' =>
+                  dlet sum := p0 + q0 in
+                  sum :: add_lists p' q'
+              end
+          end)
+         ((fix add_lists (p q : list Z) {struct p} : 
+           list Z :=
+             match p with
+             | [] => []
+             | p0 :: p' =>
+                 match q with
+                 | [] => []
+                 | q0 :: q' =>
+                     dlet sum := p0 + q0 in
+                     sum :: add_lists p' q'
+                 end
+             end)
+            (dlet sum := a0 + b0 in
+             sum
+             :: (dlet sum0 := a1 + b1 in
+                 sum0 :: (dlet sum1 := a2 + b2 in
+                          [sum1])))
+            (dlet sum := a0 + b0 in
+             sum
+             :: (dlet sum0 := a1 + b1 in
+                 sum0 :: (dlet sum1 := a2 + b2 in
+                          [sum1]))))
+         ((fix add_lists (p q : list Z) {struct p} : 
+           list Z :=
+             match p with
+             | [] => []
+             | p0 :: p' =>
+                 match q with
+                 | [] => []
+                 | q0 :: q' =>
+                     dlet sum := p0 + q0 in
+                     sum :: add_lists p' q'
+                 end
+             end)
+            (dlet sum := a0 + b0 in
+             sum
+             :: (dlet sum0 := a1 + b1 in
+                 sum0 :: (dlet sum1 := a2 + b2 in
+                          [sum1])))
+            (dlet sum := a0 + b0 in
+             sum
+             :: (dlet sum0 := a1 + b1 in
+                 sum0 :: (dlet sum1 := a2 + b2 in
+                          [sum1]))))
+```
+
+Not so great. Because the `dlet`s are stuck in the inner terms, we
+can't simplify the expression very nicely. Let's try that on the CPS
+version (`Eval cbv -[Let_In Z.add] in y`):
+
+```
+fun a0 a1 a2 b0 b1 b2 : Z =>
+       dlet sum := a0 + b0 in
+       dlet sum0 := a1 + b1 in
+       dlet sum1 := a2 + b2 in
+       dlet sum2 := sum + sum in
+       dlet sum3 := sum0 + sum0 in
+       dlet sum4 := sum1 + sum1 in
+       dlet sum5 := sum2 + sum2 in
+       dlet sum6 := sum3 + sum3 in
+       dlet sum7 := sum4 + sum4 in
+       [sum5; sum6; sum7]
+```
+
+Isn't that lovely? Since we can push continuation functions "under"
+the `dlet`s, we can end up with a nice, concise, simplified
+expression.
+
+One might suggest that we could just inline the `dlet`s and do common
+subexpression elimination. But some of our terms have so many `dlet`s
+that inlining them all would make a term too huge to process in
+reasonable time, so this is not really an option.
+
+*****)
+
+
 Local Ltac prove_id :=
   repeat match goal with
          | _ => progress intros
@@ -63,66 +306,78 @@ Module B.
 
     Definition multerm (t t' : limb) : limb :=
       (fst t * fst t', (snd t * snd t')%RT).
-    Definition mul_cps (p q:list limb) {T} (f : list limb->T) :=
-      flat_map_cps (fun t => @map_cps _ _ (multerm t) q) p f.
-    Definition mul (p q:list limb) := mul_cps p q id.
-    Hint Opaque mul : uncps.
-    Lemma eval_map_mul (a:limb) (q:list limb) : eval (List.map (multerm a) q) = fst a * snd a * eval q.
+    Lemma eval_map_multerm (a:limb) (q:list limb)
+      : eval (List.map (multerm a) q) = fst a * snd a * eval q.
     Proof.
       induction q; cbv [multerm]; simpl List.map;
         autorewrite with push_basesystem_eval cancel_pair; nsatz.
-    Qed. Hint Rewrite eval_map_mul : push_basesystem_eval.
-    Lemma mul_cps_id p q: forall {T} f,
-      @mul_cps p q T f = f (mul p q).
-    Proof. cbv [mul_cps mul]; prove_id. Qed. Hint Rewrite mul_cps_id : uncps.
-    Lemma eval_mul_noncps p q:
-      eval (mul p q) = eval p * eval q.
-    Proof.
-      cbv [mul mul_cps]; induction p; prove_eval. Qed. Hint Rewrite eval_mul_noncps : push_basesystem_eval.
+    Qed. Hint Rewrite eval_map_multerm : push_basesystem_eval.
 
-    Fixpoint split (s:Z) (xs:list limb)
+    Definition mul_cps (p q:list limb) {T} (f : list limb->T) :=
+      flat_map_cps (fun t => @map_cps _ _ (multerm t) q) p f.
+
+    Definition mul (p q:list limb) := mul_cps p q id.
+    Lemma mul_cps_id p q: forall {T} f, @mul_cps p q T f = f (mul p q).
+    Proof. cbv [mul_cps mul]; prove_id. Qed.
+    Hint Opaque mul : uncps.
+    Hint Rewrite mul_cps_id : uncps.
+
+    Lemma eval_mul p q: eval (mul p q) = eval p * eval q.
+    Proof. cbv [mul mul_cps]; induction p; prove_eval. Qed.
+    Hint Rewrite eval_mul : push_basesystem_eval.
+
+    Fixpoint split_cps (s:Z) (xs:list limb)
              {T} (f :list limb*list limb->T) :=
       match xs with
       | nil => f (nil, nil)
       | cons x xs' =>
-        split s xs'
+        split_cps s xs'
               (fun sxs' =>
         if dec (fst x mod s = 0)
         then f (fst sxs',          cons (fst x / s, snd x) (snd sxs'))
         else f (cons x (fst sxs'), snd sxs'))
       end.
-    Definition split_noncps s xs := split s xs id.
-    Hint Opaque split_noncps : uncps.
-    Lemma split_id s p: forall {T} f,
-        @split s p T f = f (split_noncps s p).
+
+    Definition split s xs := split_cps s xs id.
+    Lemma split_cps_id s p: forall {T} f,
+        @split_cps s p T f = f (split s p).
     Proof.
       induction p;
         repeat match goal with
                | _ => rewrite IHp
-               | _ => progress (cbv [split_noncps]; prove_id)
+               | _ => progress (cbv [split]; prove_id)
                end.
-    Qed. Hint Rewrite split_id : uncps.
-    Lemma eval_split_noncps s p (s_nonzero:s<>0):
-      eval (fst (split_noncps s p)) + s*eval (snd (split_noncps s p))  = eval p.
+    Qed.
+    Hint Opaque split : uncps.
+    Hint Rewrite split_cps_id : uncps.
+
+    Lemma eval_split s p (s_nonzero:s<>0):
+      eval (fst (split s p)) + s*eval (snd (split s p)) = eval p.
     Proof.
-      cbv [split_noncps];  induction p; prove_eval.
-        match goal with H:_ |- _ =>
-                        unique pose proof (Z_div_exact_full_2 _ _ s_nonzero H)
+      cbv [split];  induction p; prove_eval.
+      match goal with
+        H:_ |- _ =>
+        unique pose proof (Z_div_exact_full_2 _ _ s_nonzero H)
         end; nsatz.
-    Qed. Hint Rewrite @eval_split_noncps using auto : push_basesystem_eval.
+    Qed. Hint Rewrite @eval_split using auto : push_basesystem_eval.
 
     Definition reduce_cps (s:Z) (c:list limb) (p:list limb)
                {T} (f : list limb->T) :=
-      split s p (fun ab =>mul_cps c (snd ab) (fun rr =>f (fst ab ++ rr))).
+      split_cps s p
+                (fun ab => mul_cps c (snd ab)
+                                  (fun rr =>f (fst ab ++ rr))).
+
     Definition reduce s c p := reduce_cps s c p id.
+    Lemma reduce_cps_id s c p {T} f:
+      @reduce_cps s c p T f = f (reduce s c p).
+    Proof. cbv [reduce_cps reduce]; prove_id. Qed.
     Hint Opaque reduce : uncps.
+    Hint Rewrite reduce_cps_id : uncps.
+    
     Lemma reduction_rule a b s c (modulus_nonzero:s-c<>0) :
       (a + s * b) mod (s - c) = (a + c * b) mod (s - c).
     Proof. replace (a + s * b) with ((a + c*b) + b*(s-c)) by nsatz.
            rewrite Z.add_mod, Z_mod_mult, Z.add_0_r, Z.mod_mod; trivial. Qed.
-    Lemma reduce_cps_id s c p {T} f:
-      @reduce_cps s c p T f = f (reduce s c p).
-    Proof. cbv [reduce_cps reduce]; prove_id. Qed. Hint Rewrite reduce_cps_id : uncps.
     Lemma eval_reduce s c p (s_nonzero:s<>0) (modulus_nonzero:s-eval c<>0):
       eval (reduce s c p) mod (s - eval c) = eval p mod (s - eval c).
     Proof.
@@ -140,16 +395,16 @@ Module B.
         then dlet t2 := snd t in
              f ((w*fw, div t2 fw) :: (w, modulo t2 fw) :: @nil limb)
         else f [t].
-      Definition carry_cps(w fw:Z) (p:list limb) {T} (f:list limb->T) :=
-        flat_map_cps (carryterm_cps w fw) p f.
+
       Definition carryterm w fw t := carryterm_cps w fw t id.
-      Hint Opaque carryterm : uncps.
-      Definition carry w fw p := carry_cps w fw p id.
-      Hint Opaque carry : uncps.
       Lemma carryterm_cps_id w fw t {T} f :
         @carryterm_cps w fw t T f
         = f (@carryterm w fw t).
-      Proof. cbv [carryterm_cps carryterm Let_In]; prove_id. Qed. Hint Rewrite carryterm_cps_id : uncps.
+      Proof. cbv [carryterm_cps carryterm Let_In]; prove_id. Qed.
+      Hint Opaque carryterm : uncps.
+      Hint Rewrite carryterm_cps_id : uncps.
+
+
       Lemma eval_carryterm w fw (t:limb) (fw_nonzero:fw<>0):
         eval (carryterm w fw t) = eval [t].
       Proof.
@@ -157,10 +412,17 @@ Module B.
         specialize (div_mod (snd t) fw fw_nonzero).
         nsatz.
       Qed. Hint Rewrite eval_carryterm using auto : push_basesystem_eval.
+
+      Definition carry_cps(w fw:Z) (p:list limb) {T} (f:list limb->T) :=
+        flat_map_cps (carryterm_cps w fw) p f.
+
+      Definition carry w fw p := carry_cps w fw p id.
       Lemma carry_cps_id w fw p {T} f:
         @carry_cps w fw p T f = f (carry w fw p).
       Proof. cbv [carry_cps carry]; prove_id. Qed.
+      Hint Opaque carry : uncps.
       Hint Rewrite carry_cps_id : uncps.
+
       Lemma eval_carry w fw p (fw_nonzero:fw<>0):
         eval (carry w fw p) = eval p.
       Proof. cbv [carry_cps carry]; induction p; prove_eval. Qed.
@@ -179,17 +441,17 @@ Module B.
       Definition sat_multerm_cps (t t' : limb) {T} (f:list limb->T) :=
         dlet tt' := mul (snd t) (snd t') in
               f ((fst t*fst t', runtime_fst tt') :: (fst t*fst t'*word_max, runtime_snd tt') :: nil)%list.
-      Definition sat_mul_cps (p q : list limb) {T} (f:list limb->T) := 
-        flat_map_cps (fun t => @flat_map_cps _ _ (sat_multerm_cps t) q) p f.
-      (* TODO (jgross): kind of an interesting behavior--it infers the type arguments like this but fails to check if I leave them implicit *)
+
       Definition sat_multerm t t' := sat_multerm_cps t t' id.
-      Definition sat_mul p q := sat_mul_cps p q id.
-      Hint Opaque sat_multerm sat_mul : uncps.
       Lemma sat_multerm_cps_id t t' : forall {T} (f:list limb->T),
        sat_multerm_cps t t' f = f (sat_multerm t t').
-      Proof. reflexivity. Qed. Hint Rewrite sat_multerm_cps_id : uncps.
+      Proof. reflexivity. Qed.
+      Hint Opaque sat_multerm : uncps.
+      Hint Rewrite sat_multerm_cps_id : uncps.
+
       Lemma eval_map_sat_multerm_cps t q :
-        eval (flat_map (fun x => sat_multerm_cps t x id) q) = fst t * snd t * eval q.
+        eval (flat_map (fun x => sat_multerm_cps t x id) q)
+        = fst t * snd t * eval q.
       Proof.
         cbv [sat_multerm sat_multerm_cps Let_In runtime_fst runtime_snd];
         induction q; prove_eval;
@@ -197,8 +459,19 @@ Module B.
                               specialize (mul_correct a b) end;
           nsatz.
       Qed. Hint Rewrite eval_map_sat_multerm_cps : push_basesystem_eval.
-      Lemma sat_mul_cps_id p q {T} f : @sat_mul_cps p q T f = f (sat_mul p q).
-      Proof. cbv [sat_mul_cps sat_mul]; prove_id. Qed. Hint Rewrite sat_mul_cps_id : uncps.
+
+      Definition sat_mul_cps (p q : list limb) {T} (f:list limb->T) := 
+        flat_map_cps (fun t =>
+                        @flat_map_cps _ _ (sat_multerm_cps t) q) p f.
+      (* TODO (jgross): kind of an interesting behavior--it infers the type arguments like this but fails to check if I leave them implicit *)
+      
+      Definition sat_mul p q := sat_mul_cps p q id.
+      Lemma sat_mul_cps_id p q {T} f :
+        @sat_mul_cps p q T f = f (sat_mul p q).
+      Proof. cbv [sat_mul_cps sat_mul]; prove_id. Qed.
+      Hint Opaque sat_mul : uncps.
+      Hint Rewrite sat_mul_cps_id : uncps.
+      
       Lemma eval_sat_mul p q : eval (sat_mul p q) = eval p * eval q.
       Proof. cbv [sat_mul_cps sat_mul]; induction p; prove_eval. Qed.
       Hint Rewrite eval_sat_mul : push_basesystem_eval.
@@ -211,7 +484,7 @@ Module B.
       @Associational.carry_cps_id
       @Associational.carryterm_cps_id
       @Associational.reduce_cps_id
-      @Associational.split_id
+      @Associational.split_cps_id
       @Associational.mul_cps_id : uncps.
 
   Module Positional.
@@ -222,22 +495,28 @@ Module B.
               (weight_nonzero : forall i, weight i <> 0).
 
       (** Converting from positional to associational *)
-
       Definition to_associational_cps {n:nat} (xs:tuple Z n)
                  {T} (f:list limb->T) :=
         map_cps weight (seq 0 n)
                 (fun r =>
                    to_list_cps n xs (fun rr => combine_cps r rr f)).
-      Definition to_associational {n} xs := @to_associational_cps n xs _ id.
-      Definition eval {n} x := @to_associational_cps n x _ Associational.eval.
+      
+      Definition to_associational {n} xs :=
+        @to_associational_cps n xs _ id.
       Lemma to_associational_cps_id {n} x {T} f:
         @to_associational_cps n x T f = f (to_associational x).
       Proof. cbv [to_associational_cps to_associational]; prove_id. Qed.
+      Hint Opaque to_associational : uncps.
       Hint Rewrite @to_associational_cps_id : uncps.
+
+      Definition eval {n} x :=
+        @to_associational_cps n x _ Associational.eval.
+
       Lemma eval_to_associational {n} x :
         Associational.eval (@to_associational n x) = eval x.
-      Proof. cbv [to_associational_cps eval to_associational]; prove_eval. Qed.
-      Hint Rewrite @eval_to_associational : push_basesystem_eval.
+      Proof.
+        cbv [to_associational_cps eval to_associational]; prove_eval.
+      Qed. Hint Rewrite @eval_to_associational : push_basesystem_eval.
 
       (** Converting from associational to positional *)
 
@@ -252,8 +531,8 @@ Module B.
 
       Definition add_to_nth_cps {n} i x t {T} (f:tuple Z n->T) :=
         @on_tuple_cps _ _ 0 (update_nth_cps i (runtime_add x)) n n t _ f.
+      
       Definition add_to_nth {n} i x t := @add_to_nth_cps n i x t _ id.
-      Hint Opaque add_to_nth : uncps.
       Lemma add_to_nth_cps_id {n} i x xs {T} f:
         @add_to_nth_cps n i x xs T f = f (add_to_nth i x xs).
       Proof.
@@ -261,7 +540,10 @@ Module B.
           by (intros; autorewrite with uncps; reflexivity); prove_id.
         Unshelve.
         intros; subst. autorewrite with uncps push_id. distr_length.
-      Qed. Hint Rewrite @add_to_nth_cps_id : uncps.
+      Qed.
+      Hint Opaque add_to_nth : uncps.
+      Hint Rewrite @add_to_nth_cps_id : uncps.
+      
       Lemma eval_add_to_nth {n} (i:nat) (x:Z) (H:(i<n)%nat) (xs:tuple Z n):
         eval (@add_to_nth n i x xs) = weight i * x + eval xs.
       Proof.
@@ -287,52 +569,77 @@ Module B.
         if dec (fst t mod weight i = 0)
         then f (i, let c := fst t / weight i in (c * snd t)%RT)
         else match i with S i' => place_cps t i' f | O => f (O, fst t * snd t)%RT end.
-      Lemma place_cps_in_range (t:limb) (n:nat) : (fst (place_cps t n id) < S n)%nat.
+
+      Definition place t i := place_cps t i id.
+      Lemma place_cps_id t i {T} f :
+        @place_cps t i T f = f (place t i).
+      Proof. cbv [place]; induction i; prove_id. Qed.
+      Hint Opaque place : uncps.
+      Hint Rewrite place_cps_id : uncps.
+
+      Lemma place_cps_in_range (t:limb) (n:nat)
+        : (fst (place_cps t n id) < S n)%nat.
       Proof. induction n; simpl; break_match; simpl; omega. Qed.
-      Lemma weight_place_cps t i : weight (fst (place_cps t i id)) * snd (place_cps t i id) = fst t * snd t.
+      Lemma weight_place_cps t i
+        : weight (fst (place_cps t i id)) * snd (place_cps t i id)
+          = fst t * snd t.
       Proof.
         induction i; cbv [id]; simpl place_cps; break_match;
           autorewrite with cancel_pair;
           try find_apply_lem_hyp Z_div_exact_full_2; nsatz || auto.
       Qed.
-      Definition place t i := place_cps t i id.
-      Hint Opaque place : uncps.
-      Lemma place_cps_id t i {T} f :
-        @place_cps t i T f = f (place t i).
-      Proof. cbv [place]; induction i; prove_id. Qed.
-      Hint Rewrite place_cps_id : uncps.
-      Definition from_associational_cps n (p:list limb) {T} (f:tuple Z n->T):=
-        fold_right_cps (fun t st => place_cps t (pred n) (fun p=> add_to_nth_cps (fst p) (snd p) st id)) (zeros n) p f.
+
+      Definition from_associational_cps n (p:list limb)
+                 {T} (f:tuple Z n->T):=
+        fold_right_cps
+          (fun t st =>
+             place_cps t (pred n)
+                       (fun p=> add_to_nth_cps (fst p) (snd p) st id))
+          (zeros n) p f.
+
       Definition from_associational n p := from_associational_cps n p id.
-      Hint Opaque from_associational : uncps.
       Lemma from_associational_cps_id {n} p {T} f:
         @from_associational_cps n p T f = f (from_associational n p).
-      Proof. cbv [from_associational_cps from_associational]; prove_id. Qed.
+      Proof.
+        cbv [from_associational_cps from_associational]; prove_id.
+      Qed.
+      Hint Opaque from_associational : uncps.
       Hint Rewrite @from_associational_cps_id : uncps.
+
       Lemma eval_from_associational {n} p (n_nonzero:n<>O):
         eval (from_associational n p) = Associational.eval p.
       Proof.
         cbv [from_associational_cps from_associational]; induction p;
           [|pose proof (place_cps_in_range a (pred n))]; prove_eval.
         cbv [place]; rewrite weight_place_cps. nsatz.
-      Qed. Hint Rewrite @eval_from_associational using omega : push_basesystem_eval.
+      Qed.
+      Hint Rewrite @eval_from_associational using omega
+        : push_basesystem_eval.
 
       Section Carries.
         Context {modulo div : Z->Z->Z}.
         Context {div_mod : forall a b:Z, b <> 0 ->
                                        a = b * (div a b) + modulo a b}.
-      Definition carry_cps(index:nat) (p:list limb) {T} (f:list limb->T) :=
-        @Associational.carry_cps modulo div (weight index) (weight (S index) / weight index) p T f.
+        Definition carry_cps(index:nat) (p:list limb)
+                   {T} (f:list limb->T) :=
+          @Associational.carry_cps modulo div
+                                   (weight index)
+                                   (weight (S index) / weight index)
+                                   p T f.
+
       Definition carry i p := carry_cps i p id.
-      Hint Opaque carry : uncps.
       Lemma carry_cps_id i p {T} f:
         @carry_cps i p T f = f (carry i p).
-      Proof. cbv [carry_cps carry]; prove_id; rewrite carry_cps_id; reflexivity. Qed.
-      Hint Rewrite carry_cps_id : uncps.
+      Proof.
+        cbv [carry_cps carry]; prove_id; rewrite carry_cps_id; reflexivity.
+      Qed.
+      Hint Opaque carry : uncps. Hint Rewrite carry_cps_id : uncps.
+
       Lemma eval_carry i p: weight (S i) / weight i <> 0 ->
         Associational.eval (carry i p) = Associational.eval p.
       Proof. cbv [carry_cps carry]; intros; eapply @eval_carry; eauto. Qed.
       Hint Rewrite @eval_carry : push_basesystem_eval.
+
       End Carries.
     End Positional.
   End Positional.
@@ -342,7 +649,7 @@ Module B.
       @Associational.carry_cps_id
       @Associational.carryterm_cps_id
       @Associational.reduce_cps_id
-      @Associational.split_id
+      @Associational.split_cps_id
       @Associational.mul_cps_id
       @Positional.carry_cps_id
       @Positional.from_associational_cps_id
@@ -352,12 +659,12 @@ Module B.
     : uncps.
   Hint Rewrite
       @Associational.eval_sat_mul
-      @Associational.eval_mul_noncps
+      @Associational.eval_mul
       @Positional.eval_to_associational
       @Associational.eval_carry
       @Associational.eval_carryterm
       @Associational.eval_reduce
-      @Associational.eval_split_noncps
+      @Associational.eval_split
       @Positional.eval_carry
       @Positional.eval_from_associational
       @Positional.eval_add_to_nth
